updates

Main.lean
@@ -1,4 +1,81 @@
+
 import Jax
+
 
 def main : IO Unit :=
   IO.println s!"Hello, {hello}!"
+
+def alpha : Nat := 1
+
+
+
+inductive type
+| base : string -> type
+| arrow : type -> type -> type
+
+inductive term
+| const : type -> term
+| var : string -> term
+| abstraction : string -> type -> term -> term
+| apply : term -> term -> term
+
+@[reducible] def context :=
+  List (String × type)
+
+def lookup : context -> string -> option type
+| [] _ => none
+| ((n, t) :: delta) n' =>
+  if n = n'
+  then some t
+  else none
+
+inductive typed : context -> term -> type -> Prop
+| well_typed_var :
+  forall ctxt n t,
+    lookup ctxt n = some t ->
+    typed ctxt (term.var n) t
+| well_typed_const :
+  forall ctxt T,
+    typed ctxt (term.const T) T
+| well_typed_abs :
+  forall ctxt n tA tB body,
+    typed ((n, tA) :: ctxt) body tB ->
+    typed ctxt (term.abstraction n tA body) (type.arrow tA tB)
+| well_typed_apply :
+  forall ctxt f arg tA tB,
+    typed ctxt f (type.arrow tA tB) ->
+    typed ctxt arg tA ->
+    typed ctxt (term.apply f arg) tB
+
+inductive value : term -> Prop
+
+inductive subst : term → term → string → term → Prop
+| const : forall T e x, subst (term.const T) e x (term.const T)
+| var_equal :
+  forall x e,
+    subst (term.var x) e x e
+| var_else :
+  forall x x' e,
+    not (x = x') ->
+    subst (term.var x) e x' (term.var x)
+| abs_equal :
+  forall x t e body,
+    subst (term.abstraction x t body) e x (term.abstraction x t body)
+| abs_else :
+  forall x x' t e body body',
+    not (x = x') ->
+    subst body e x' body' ->
+    subst (term.abstraction x t body) e x' (term.abstraction x t body')
+| app : forall x e f f' g g',
+  subst f e x f' ->
+  subst g e x g' ->
+  subst (term.apply f g) e x (term.apply f' g')
+
+lemma subst_deterministic :
+  ∀ e1 e2 x e3,
+  subst e1 e2 x e3 ->
+    ∀ e3',
+    subst e1 e2 x e3' ->
+    e3 = e3' :=
+begin
+  
